debug pattern matching when no forall

theories/elimination_pattern_matching.v
@@ -94,13 +94,6 @@ match goal with
 | _ => n
 end in revert_count_rec 0.
 
-Ltac is_a_variable x :=
-let x':= metacoq_get_value (tmQuote x) in 
-match x' with 
-| tVar _ => idtac
-| _ => fail
-end.
-
 Ltac contains t u :=
 match t with
 | context [u] => idtac
@@ -123,20 +116,35 @@ Ltac elim_match_with_no_forall H :=
     let foo := fresh in 
     assert (foo : False -> U) 
 by (let Hfalse := fresh in
-intro Hfalse ; tryif (is_a_variable expr)
-then (case expr)
-else (case_eq expr) ;
+intro Hfalse ; 
+(case_eq expr) ;
 match goal with 
 | u : Prop |- ?G => instantiate (u := G); destruct Hfalse
 end) ; clear foo ; 
 repeat match goal with 
-| u : Prop |-_ => let H0 := fresh in let u' := eval unfold u in u in assert (H0 : u')  by 
+| u : Prop |-_ => let H0 := fresh in let u' := eval unfold u in u in assert (H0 : u')   by 
 (first [ try (rewrite H); reflexivity
 |intros ; match goal with 
 | Hinv : _ |- _ => rewrite Hinv in H ; auto
 end]); try elim_match_with_no_forall H0 ; clear u 
 end
 end ; clear H.
+
+(* Tests *)
+
+Fixpoint leb (n:nat)(m:nat) :=
+  match n,m with
+  | 0,_ => true
+  | (S _) , 0  => false
+  | S n, S m => leb n m
+  end.
+
+Lemma leb_le : forall n m, (leb n m = true) -> le n m.
+  intros n. induction n. intros m.
+  intros H. induction m.
+  constructor. constructor. apply IHm.
+  constructor. intros m. intro H. simpl in H.  
+  elim_match_with_no_forall H. Abort.
 
 
 Ltac eliminate_dependent_pattern_matching H :=
